hMul for symbols and words, additional definitions from L1

FormaleSystemeInLean/LectureAndExercise/lecture1.lean
@@ -1,6 +1,27 @@
 
 def Set (α : Type u) := α -> Prop
 
+-- inspired by mathlib
+class Fintype (α : Type u) where
+  elems : List α
+  complete : ∀ a : α, a ∈ elems
+
+/-
+
+Leeres Wort: Länge 0 -> kann man dafür das symbol ε reservieren?
+Neutrales Element der konkatenation für Wörter (ist das Definition oder muss man das beweisen? )
+Präfix
+Infix
+Suffix
+Sprache: Menge von Wörtern über Alphabet
+Kleinste sprache: leere sprache
+Teilmenge jeder anderen sprache
+Größte Sprache: Sigma Stern
+Jede sprache über sigma ist Teilmenge davon
+
+-/
+
+
 -- The following type class instances are just allowing us to use some basic notation like ∅, ∈ or ∪ with the right definitions..
 instance : EmptyCollection (Set α) where
   emptyCollection := fun _ => False
@@ -20,27 +41,79 @@ instance : HasSubset (Set α) where
 instance : HasSSubset (Set α) where
   SSubset A B := A ⊆ B ∧ ¬ B ⊆ A
 
+instance : SDiff (Set α) where
+  sdiff A B := fun e => e ∈ A ∧ ¬(e ∈ B)
+
 -- Set extensionality: Two sets are equal if they contain the same elements. This is not something we define but we can prove it!
 theorem Set.ext (X Y : Set α) : (∀ e, e ∈ X ↔ e ∈ Y) -> X = Y := by
   intro h; apply funext; intro e; apply propext; specialize h e; exact h
 
+-- From now on, we pick some alphabet Sigma. In fact, we do not even care about the type of Sigma. In can basically be anything.
+variable {Sigma : Type u}
 
 -- Words are merely lists over some alphabet Sigma. In fact, we do not even care about the type of Sigma.
 abbrev Word (Sigma : Type u) := List Sigma
 
--- A language is in turn just a set of words.
-abbrev Language (Sigma : Type u) := Set (Word Sigma)
+-- Example:
+def Alphabet : Set Char := fun σ : Char => σ = 'a' ∨ σ = 'b'
 
--- From now on, we pick some alphabet Sigma. In fact, we do not even care about the type of Sigma. In can basically be anything.
-variable {Sigma : Type u}
+-- Words: Properties and Operations (Slides 29-...)
 
 -- Let's define concatenation as multiplication.
 instance : Mul (Word Sigma) where
   mul u v := List.append u v
 
--- Also for Languages
+instance [BEq Sigma] : HMul Sigma (Word Sigma) (Word Sigma) where
+  hMul σ w := List.insert σ w
+
+-- Examples
+#eval ['a','b'] * ['b','a']
+
+def some_word : Word Char := ['S','t','a','u','b','e','c','k','e','n']
+
+#eval List.IsPrefix ['S','t','a','u','b'] some_word
+--#eval List.IsInfix ['t','a','u','b'] some_word
+#eval List.IsSuffix ['e','c','k','e','n'] some_word
+
+#eval 'a'::some_word
+
+-- für alle alphabete sigma existiert ein leeres wort []
+-- [] * w = w für alle w ∈ sigma* (mit List.concat ?)
+
+-- evtl.: für alle nichtleeren wörter gilt: w = u*v (v darf leer sein)
+-- kann man zeigen: head::tail = head * tail ?
+
+theorem nonempty_prefix [BEq Sigma] (σ : Sigma) (w : Word Sigma) : σ::w = σ * w := by
+
+  sorry
+
+theorem epsilon_concat : ∀ (w : Word Sigma), w * [] = w := by
+  intro w
+  induction w with
+  | nil =>
+    trivial
+  | cons σ u ih =>
+
+    sorry
+
+
+-- A language is in turn just a set of words.
+abbrev Language (Sigma : Type u) := Set (Word Sigma)
+
+-- The "biggest language" Σ* contains all words over Σ
+def sigma_star : Language Sigma := fun w : Word Sigma => True
+
+-- Every language over Σ is a subset of Σ*
+theorem sigma_star_subset : ∀ (L: Language Sigma), L ⊆ sigma_star := by
+  sorry
+
+-- Concatenation of Languages
 instance : Mul (Language Sigma) where
   mul L1 L2 := fun w => ∃ u ∈ L1, ∃ v ∈ L2, w = u * v
+
+-- Complement
+def Language.complement (L : Language Sigma) : Language Sigma :=
+  sigma_star \ L
 
 -- For languages we can also execute concatenation multiple times and define this via Powers.
 def Language.pow (L : Language Sigma) : Nat -> Language Sigma
